src/myprime.lean
@@ -47,12 +47,38 @@ existsi p,trace_state,
   trace_state,
   have pp : prime p, from min_fac_prime f1,
 split,
+trace_state,
 { apply le_of_not_ge,
+  trace_state,
+  trace_goals,
   intro h,
+  trace_goals,
+  trace_state,
   have h₁ : p ∣ n!, from dvd_factorial (min_fac_pos _) h,
+  trace_state,
   have h₂ : p ∣ 1, from (nat.dvd_add_iff_right h₁).2 (min_fac_dvd _),
   from  prime.not_dvd_one pp h₂,
 },
 T,{assumption}
+,trace_state
+end
+
+theorem exists_infinite_primes5 (n : ℕ) : ∃ p, n ≤ p ∧ prime p :=
+begin[ntac]
+let p := min_fac (n! + 1),trace_state,
+existsi p,trace_state,
+  have f1 : n! + 1 ≠ 1,
+  trace_state,
+  from (ne_of_gt $ succ_lt_succ $ factorial_pos n),
+  trace_state,
+  suffices hh: n ≤ p, from ⟨hh, min_fac_prime f1⟩,
+{trace_state,
+  by_contradiction,trace_state,
+  simp at h,trace_state,
+  have h1: p ≤ n, from le_of_lt h,
+  have h₁ : p ∣ n!, from dvd_factorial (min_fac_pos _) h1,
+  have h₂ : p ∣ 1, from (nat.dvd_add_iff_right h₁).2 (min_fac_dvd _),
+  from  prime.not_dvd_one (min_fac_prime f1) h₂,
+}
 ,trace_state
 end
