src/ntac/default.lean
@@ -1,2 +1,1 @@
-import ntac.ntac
 import ntac.interactive
