src/ntac/semantic_tree.lean
@@ -1,20 +1,26 @@
-inductive prop : Type
-| noun : prop
+import ntac.statement
+
 
 meta inductive semantic_tree : Type
 | assume_prop : expr → semantic_tree → semantic_tree
-| assume_var : expr → semantic_tree → semantic_tree
+| assume_val : expr → expr → semantic_tree → semantic_tree
 | but_false : semantic_tree → semantic_tree
 | assume_exist : expr → semantic_tree → semantic_tree
-| have_from : prop → prop → semantic_tree → semantic_tree
-| have_triv : prop → semantic_tree
-| suffice : prop → semantic_tree → semantic_tree
+| have_exact : expr → semantic_tree → semantic_tree
+| have_from : semantic_tree → semantic_tree → semantic_tree
+| let_from : semantic_tree → semantic_tree → semantic_tree
+| have_triv : expr → semantic_tree
+| suffice_from : expr → semantic_tree → semantic_tree → semantic_tree
+| exact : expr → semantic_tree
 | trivial : semantic_tree
+| unresolved : semantic_tree
+| contra : semantic_tree → semantic_tree
+| init : semantic_tree → semantic_tree
 
-meta def semantic_tree_to_string : semantic_tree → string :=
+meta def semantic_tree_to_list_statement : semantic_tree → list statement :=
 λ s,match s with
-| semantic_tree.trivial := "gtg"
-| semantic_tree.suffice p s := "dfdfd"
+| semantic_tree.trivial := [statement.trivial]
+| semantic_tree.suffice_from p s := "dfdfd"
 | semantic_tree.have_from p v s := "df"
 | _ := "fg"
   end
