src/ntac/statement.lean
@@ -1,5 +1,7 @@
 inductive prop : Type
 | noun : prop
 
-meta inductive sentence_tree : Type
-| this
+meta inductive statement : Type
+| trivial : statement
+
+
